Capless/WellScoped/Basic.lean
@@ -1,5 +1,6 @@
 import Capless.Store
 import Capless.Subcapturing
+import Capless.Subcapturing.Basic
 import Capless.Inversion.Context
 
 /-!
@@ -20,6 +21,7 @@ theorem WellScoped.proj (hsc : WellScoped Γ cont C) : WellScoped Γ cont (C.pro
   case ckind hb hw => apply ckind hb hw.proj
   case label hb hl hw => apply label hb hl hw.proj
   case label_disj hb hd hw => apply label_disj hb hd hw.there
+  case label_absurd hb ha => apply label_absurd hb ha.there
 
 theorem WellScoped.subset {C1 C2 : CaptureSet n k}
   (hsc : WellScoped Γ cont C2)
@@ -52,6 +54,7 @@ theorem WellScoped.cons
     apply hw
   case label_disj hb hd =>
     apply! label_disj
+  case label_absurd => apply! label_absurd
 
 theorem WellScoped.conse
   (hsc : WellScoped Γ cont C) :
@@ -68,6 +71,7 @@ theorem WellScoped.conse
     constructor; assumption
     apply hw
   case label_disj => apply! label_disj
+  case label_absurd => apply! label_absurd
 
 theorem WellScoped.scope
   (hsc : WellScoped Γ cont C) :
@@ -84,15 +88,16 @@ theorem WellScoped.scope
     constructor; assumption
     apply hw
   case label_disj => apply! label_disj
+  case label_absurd => apply! label_absurd
 
 theorem WellScoped.subkind' {C D : CaptureSet n k}
   (hsc : WellScoped Γ cont D)
   (heq : D = C.proj K2)
   (hs : K1.Subkind K2)
   : WellScoped Γ cont (C.proj K1) := by
-  induction hsc <;> (unfold CaptureSet.proj at heq; split at heq <;> simp at heq; simp)
+  induction hsc generalizing C <;> (unfold CaptureSet.proj at heq; split at heq <;> simp at heq; simp)
   { apply empty }
-  { have ⟨_, _⟩ := heq; subst_vars; simp_all
+  { have ⟨_, _⟩ := heq; subst_vars;
     rename_i ih1 _ ih2
     apply union (ih1 _) (ih2 _) <;> rfl }
   { subst_vars
@@ -115,22 +120,96 @@ theorem WellScoped.subkind' {C D : CaptureSet n k}
     rfl }
   { subst_vars
     rename_i hw
-    apply! ckind _ hw.proj_inv.proj
-  }
+    apply! ckind _ hw.proj_inv.proj }
   { subst_vars
     rename_i hw
-    apply! label _ _ hw.proj_inv.proj
-  }
+    apply! label _ _ hw.proj_inv.proj }
   { subst_vars
     rename_i hw
     cases hw
     case here hw => apply! label_disj _ (hw.refine_by_subkind _) (.here _)
-    case there hw => apply! label_disj _ _ (.there _)
-  }
+    case there hw => apply! label_disj _ _ (.there _) }
+  { subst_vars
+    rename_i hb _ _ hw
+    cases hw
+    case here hd hw =>
+      apply label_absurd hb (.here _ hw)
+      apply! (hd.symm.refine_by_subkind _).symm
+    case there hw => apply! label_absurd hb (.there _) }
 
 theorem WellScoped.subkind {C: CaptureSet n k} (hsc : WellScoped Γ cont (C.proj K2)) (hs : K1.Subkind K2) : WellScoped Γ cont (C.proj K1) := by
   apply subkind' hsc _ hs
   rfl
+
+-- theorem WellScoped.capture_kind'
+--   (hsc : WellScoped Γ cont D)
+--   (heq : D = C.proj K)
+--   (hk : CaptureKind Γ C K)
+--   : WellScoped Γ cont C := by
+--   induction hsc generalizing C <;> (unfold CaptureSet.proj at heq; split at heq <;> simp at heq)
+--   { apply empty }
+--   { have ⟨_, _⟩ := heq; subst_vars
+--     rename_i h1 ih1 h2 ih2
+--     have ⟨_, _⟩ := hk.union_l_inv
+--     -- apply union (ih1 _ hk) (ih2 _ hk)
+--     apply! union (ih1 (.refl _) _) (ih2 (.refl _) _) }
+--   { rename_i hb hw hsc ih _ _;
+--     subst_vars;
+--     cases hw;
+--     apply singleton hb
+--     assumption
+--     apply ih (.refl _)
+--     apply hk.widen_var hb
+--     assumption }
+--   { rename_i hb hw hsc ih _ _;
+--     subst_vars;
+--     cases hw;
+--     apply csingleton hb
+--     assumption
+--     apply ih (.refl _)
+--     apply hk.widen_cinstr hb
+--     assumption }
+--   { rename_i hb hw hsc ih _ _;
+--     subst_vars;
+--     cases hw;
+--     apply cbound hb
+--     assumption
+--     apply ih (.refl _)
+--     apply hk.widen_cbound hb
+--     assumption }
+--   { rename_i hb hi _ _
+--     cases hi <;> cases heq
+--     apply! ckind
+--   }
+--   { rename_i hb hl hi _ _
+--     cases hi <;> cases heq
+--     apply! label }
+--   { rename_i hb hd hi _ _
+--     cases hi <;> cases heq
+--     case here.refl hi =>
+--       cases hk.widen_lbound hb hi
+--       case inl hsub => cases Kind.subkind_disjoint_absurd hsub hd.symm
+--       case inr hi =>
+--         have ⟨K1, _, hi⟩ := hi
+--         apply label_disj hb _ hi
+--         apply! hd.refine_by_subkind
+--     case there.refl hi => apply! label_disj
+--   }
+
+-- theorem WellScoped.capture_kind (hsc : WellScoped Γ cont (C.proj K)) (hk : CaptureKind Γ C K) : WellScoped Γ cont C := by apply! hsc.capture_kind' $ .refl _
+
+theorem WellScoped.union_inv (hsc : WellScoped Γ cont (C1 ∪ C2)) : WellScoped Γ cont C1 ∧ WellScoped Γ cont C2 := by
+  cases hsc; aesop
+
+theorem WellScoped.singleton_inv (hsc : WellScoped Γ cont {x=x}) (hb : Γ.Bound x S^C) : WellScoped Γ cont C := by
+  cases hsc
+  case singleton hb1 hs hw => cases hw; cases Context.bound_injective hb hb1; assumption
+  case csingleton hw => cases hw
+  case cbound hw => cases hw
+  case ckind hw => cases hw
+  case label hb1 _ hw => cases hw; cases Context.bound_lbound_absurd hb hb1
+  case label_disj hb1 _ hw => cases hw
+  case label_absurd hb1 _ hw => cases hw
 
 theorem WellScoped.subcapt (hsc : WellScoped Γ cont C2) (hsub : Subcapt Γ C1 C2) : WellScoped Γ cont C1 := by
   induction hsub
@@ -142,11 +221,11 @@ theorem WellScoped.subcapt (hsc : WellScoped Γ cont C2) (hsub : Subcapt Γ C1 C
   case cinstl hb =>
     cases hsc
     case singleton hv => cases hv
-    case csingleton hb1 _ _ _ hv =>
+    case csingleton hb1 _ hv =>
       cases hv
       cases Context.cbound_injective hb1 hb
       assumption
-    case cbound hb1 _ _ _ hv =>
+    case cbound hb1 _ hv =>
       cases hv
       cases Context.cbound_injective hb1 hb
     case ckind hb1 hv =>
@@ -154,8 +233,41 @@ theorem WellScoped.subcapt (hsc : WellScoped Γ cont C2) (hsub : Subcapt Γ C1 C
       cases Context.cbound_injective hb1 hb
     case label hv => cases hv
     case label_disj hv => cases hv
-  case cinstr hb =>
-    apply csingleton hb _ _
+    case label_absurd hb ha => cases ha
+  case cinstr hb => apply! csingleton _ .var
+  case cbound hb => apply! cbound _ .var
+  case singleton_proj_sub hk =>
+    rw [← CaptureSet.proj_singleton] at hsc
+    apply! hsc.subkind
+  case singleton_proj_l => apply! hsc.proj
+  case proj_r C D K hsub hk ih =>
+    induction hk
+    case union ha hb iha ihb =>
+      have ⟨_, _⟩ := hsub.union_l_inv
+      apply union
+      { apply iha
+        assumption
+        intro cont h
+        have ⟨_, _⟩ := (ih h).union_inv
+        assumption
+        assumption }
+      { apply ihb
+        assumption
+        intro cont h
+        have ⟨_, _⟩ := (ih h).union_inv
+        assumption
+        assumption }
+    case var hb hk ih2 =>
+
+
+
+
+
+
+
+
+
+
 
 
 
